work on funcalls with mutual induction again

Simu/Cor.v
@@ -9,6 +9,7 @@ Require Import common.Separation.
 Require Import common.Values.
 Require Import common.Memory.
 Require Import common.Events.
+Require Import common.Globalenvs.
 
 Require Import Rustre.Common.
 Require Import Rustre.RMemory.
@@ -101,25 +102,24 @@ Section PRESERVATION.
   | wf_const: forall cst ty,
       well_formed_exp c m (Const cst ty).
 
-  Inductive well_formed_stmt (c: class) (m: method) (S: state): stmt -> Prop :=
+  Inductive well_formed_stmt (c: class) (m: method): stmt -> Prop :=
   | wf_assign: forall x e,
       In (x, typeof e) (meth_vars m) ->
       well_formed_exp c m e ->
-      well_formed_stmt c m S (Assign x e)
+      well_formed_stmt c m (Assign x e)
   | wf_assignst: forall x e,
       In (x, typeof e) c.(c_mems) ->
       well_formed_exp c m e ->
-      well_formed_stmt c m S (AssignSt x e)
+      well_formed_stmt c m (AssignSt x e)
   | wf_ite: forall e s1 s2,
       well_formed_exp c m e ->
-      well_formed_stmt c m S s1 ->
-      well_formed_stmt c m S s2 ->
-      well_formed_stmt c m S (Ifte e s1 s2)
-  | wf_comp: forall S' s1 s2,
-      well_formed_stmt c m S s1 ->
-      stmt_eval prog S s1 S' ->
-      well_formed_stmt c m S' s2 ->
-      well_formed_stmt c m S (Comp s1 s2)
+      well_formed_stmt c m s1 ->
+      well_formed_stmt c m s2 ->
+      well_formed_stmt c m (Ifte e s1 s2)
+  | wf_comp: forall  s1 s2,
+      well_formed_stmt c m s1 ->
+      well_formed_stmt c m s2 ->
+      well_formed_stmt c m (Comp s1 s2)
   | wf_call: forall ys clsid c' prog' o fid f es,
       (* In (y, ty) (class_vars c) -> *)
       (* Nelist.length ys = Nelist.length rvs -> *)
@@ -139,9 +139,9 @@ Section PRESERVATION.
       (* ty <> Ctypes.Tvoid -> *)
       find_class clsid prog = Some (c', prog') ->
       find_method fid (c_methods c') = Some f ->
-      well_formed_stmt c m S (Call ys clsid o fid es)
+      well_formed_stmt c m (Call ys clsid o fid es)
   | wf_skip: 
-      well_formed_stmt c m S Skip.
+      well_formed_stmt c m Skip.
   
    Remark valid_val_access:
     forall v t, valid_val v t -> access_mode t = By_value (chunk_of_type t).
@@ -181,6 +181,7 @@ Section PRESERVATION.
       le ! out_id = Some (Vptr outb Int.zero) ->
       gcenv ! (prefix f.(m_name) c.(c_name)) = Some outco ->
       sep_invariant c f S e le m sb sofs outb outco ->
+      (0 <= Int.unsigned sofs)%Z ->
       match_states c f S (e, le, m).
 
   Remark invariant_blockrep:
@@ -354,33 +355,60 @@ Section PRESERVATION.
       [now app_match_find_var_det | contradiction].
   Qed.
 
+  Remark field_offset_rec_in_range':
+    forall flds x ofs pos,
+      field_offset_rec gcenv x flds pos = Errors.OK ofs ->
+      (pos <= ofs)%Z.
+  Proof.
+    induction flds as [|[i t]]; simpl; intros.
+    - discriminate.
+    - destruct (AST.ident_eq x i); intros.
+      + inv H. apply align_le. apply alignof_pos.
+      + specializes IHflds H. eapply Zle_trans; eauto.
+        apply Zle_trans with (align pos (alignof gcenv t)).
+        * apply align_le. apply alignof_pos.
+        * generalize (sizeof_pos gcenv t). omega.
+  Qed.
+
+  Remark field_offset_in_range':
+  forall flds x ofs,
+  field_offset gcenv x flds = Errors.OK ofs ->
+  (0 <= ofs)%Z.
+  Proof.
+    unfold field_offset; intros.
+    apply* field_offset_rec_in_range'.
+  Qed.
+  
   Lemma evall_self_field:
     forall clsnm prog' c f S e le m x ty sb sofs outb outco,
       find_class clsnm prog = Some (c, prog') ->
       In f c.(c_methods) ->
       le ! self_id = Some (Vptr sb sofs) ->
+      (0 <= Int.unsigned sofs)%Z ->
       sep_invariant c f S e le m sb sofs outb outco ->
       In (x, ty) (c_mems c) ->
       exists d,
         eval_lvalue tge e le m (deref_field self_id (c_name c) x ty)
                     sb (Int.add sofs (Int.repr d))
         /\ field_offset gcenv x (make_members c) = Errors.OK d
-        /\ (0 <= Int.unsigned sofs + d <= Int.max_unsigned)%Z.
+        /\ (0 <= d <= Int.max_unsigned)%Z.
   Proof.
-    introv Find ? ? Hrep ?.
+    introv Find ? ? ? Hrep Hin.
     destruct S.
     forwards ?: find_class_name Find; subst.
     eapply invariant_staterep in Hrep; eauto.
     forwards* (? & Hco & ? & Eq & ? & ?): make_members_co; instantiate (1:=tprog) in Hco.
-    assert (In (x, ty) (make_members c)) by
-        (unfold make_members; rewrite in_app_iff; now left).
-    forwards* (d & Hoffset & ?): staterep_field_offset. 
-    exists d; split*.
-    apply* eval_Efield_struct.
-      * apply* eval_Elvalue.
+    forwards* (d & Hoffset & (Hpos & Hnotmax)): staterep_field_offset. 
+    exists d; splits*.
+    - apply* eval_Efield_struct.
+      + apply* eval_Elvalue.
         apply* deref_loc_copy. 
-      * simpl; unfold type_of_inst; eauto.
-      * rewrite* Eq. 
+      + simpl; unfold type_of_inst; eauto.
+      + rewrite* Eq. 
+    - apply* field_offset_in_range'.
+    - rewrite Z.add_comm in Hnotmax.
+      rewrite <-Z.add_0_r in Hnotmax. 
+      apply Z.le_le_add_le with (m:=Int.unsigned sofs) (n:=Z0); auto.
   Qed.
   
   Lemma eval_self_field:
@@ -388,20 +416,20 @@ Section PRESERVATION.
       find_class clsnm prog = Some (c, prog') ->
       In f c.(c_methods) ->
       le ! self_id = Some (Vptr sb sofs) ->
+      (0 <= Int.unsigned sofs)%Z ->
       sep_invariant c f S e le m sb sofs outb outco ->
       In (x, ty) (c_mems c) ->
       find_field S x v ->
       valid_val v ty ->
       eval_expr tge e le m (deref_field self_id (c_name c) x ty) v.
   Proof.
-    introv ? ? ? Hrep ? ? ?.
+    introv ? ? ? ? Hrep ? ? ?.
     destruct S.
     edestruct evall_self_field as (? & ? & Hoffset & (? & ?)); eauto.
     eapply invariant_staterep in Hrep; eauto.
     apply* eval_Elvalue.
     apply* staterep_deref_mem.
     rewrite* Int.unsigned_repr.
-    admit.
   Qed.
   
   Lemma expr_eval_simu:
@@ -498,6 +526,7 @@ Section PRESERVATION.
       le ! out_id = Some (Vptr outb Int.zero) ->
       le ! self_id = Some (Vptr sb sofs) ->
       gcenv ! (prefix (m_name f) (c_name c)) = Some outco ->
+      (0 <= Int.unsigned sofs)%Z ->
       sep_invariant c f S e le m sb sofs outb outco ->
       In (x, ty) (meth_vars f) ->
       field_offset gcenv x (co_members outco) = Errors.OK d ->
@@ -507,7 +536,7 @@ Section PRESERVATION.
       exists m', Memory.Mem.storev (chunk_of_type ty) m (Vptr outb (Int.repr d)) v = Some m'
             /\ match_states c f (update_var S x v) (e, le, m').
   Proof.
-    intros **  ? ? ? ? Houtco Hrep Hvars Hoffset Haccess Hlr E.
+    intros **  ? ? ? ? Houtco ? Hrep Hvars Hoffset Haccess Hlr E.
     destruct S.
     unfold sep_invariant in Hrep.
 
@@ -596,12 +625,13 @@ Section PRESERVATION.
       le ! out_id = Some (Vptr outb Int.zero) ->
       le ! self_id = Some (Vptr sb sofs) ->
       gcenv ! (prefix (m_name f) (c_name c)) = Some outco ->
+      (0 <= Int.unsigned sofs)%Z ->
       sep_invariant c f S e le m sb sofs outb outco ->
       In (x, ty) (meth_vars f) ->
       existsb (fun out => ident_eqb (fst out) x) f.(m_out) = false ->
       match_states c f (update_var S x v) (e, PTree.set x v le, m).
   Proof.
-    intros ** ? ? ? ? Hout Hself ? Hrep Hin E.
+    intros ** ? ? ? ? Hout Hself ? ? Hrep Hin E.
     rewrite <-PTree.gso with (j:=x) (x:=v) in Hout; auto.
     rewrite <-PTree.gso with (j:=x) (x:=v) in Hself; auto.
     eapply not_existsb_In in E; eauto.
@@ -658,12 +688,13 @@ Section PRESERVATION.
   Qed.  
 
   Lemma match_states_assign_state:
-    forall c clsnm prog' f S x ty e le m v d sb sofs outco outb,
+    forall c clsnm prog' f S x ty e le m v d sb sofs outco outb, 
       find_class clsnm prog = Some (c, prog') ->
       In f c.(c_methods) ->
       le ! out_id = Some (Vptr outb Int.zero) ->
       le ! self_id = Some (Vptr sb sofs) ->
       gcenv ! (prefix (m_name f) (c_name c)) = Some outco ->
+      (0 <= Int.unsigned sofs)%Z ->
       sep_invariant c f S e le m sb sofs outb outco ->
       In (x, ty) (c_mems c) ->
       field_offset gcenv x (make_members c) = Errors.OK d ->
@@ -671,7 +702,7 @@ Section PRESERVATION.
       exists m', Memory.Mem.storev (chunk_of_type ty) m (Vptr sb (Int.repr (Int.unsigned sofs + d))) v = Some m'
             /\ match_states c f (update_field S x v) (e, le, m').
   Proof.
-    intros **  ? ? ? ? Houtco Hrep Hmems Hoffset Hlr.
+    intros **  ? ? ? ? Houtco ? Hrep Hmems Hoffset Hlr.
     destruct S.
     unfold sep_invariant in Hrep.
     
@@ -725,26 +756,61 @@ Section PRESERVATION.
   
   (* Hint Constructors Clight.eval_lvalue Clight.eval_expr well_formed_stmt. *)
   Hint Resolve expr_eval_simu Clight.assign_loc_value exp_eval_valid sem_cast_same.
-  
-  Theorem correctness:
-    forall c prog' f s S1 S2,
-      stmt_eval prog S1 s S2 ->
-      find_class c.(c_name) prog = Some (c, prog') ->
-      In f c.(c_methods) ->
-      well_formed_stmt c f S1 s ->
-      forall e1 le1 m1,
-        match_states c f S1 (e1, le1, m1) ->
-        exists le2 m2 t,
-          exec_stmt tge (function_entry2 tge) e1 le1 m1
-                    (translate_stmt prog c f s) t le2 m2 Out_normal
-          /\ match_states c f S2 (e1, le2, m2).
-  Proof.
-    remember prog.
-    clear TRANSL main_node_exists.
-    introv EV; induction EV; introv Find HfIn WF MS; subst;
-    inversion_clear WF as [? ? Hvars|? ? Hin| | |? ? ? ? ? ? ? ? ? Find' Findmeth|];
-    pose proof MS as MS'; inverts MS' as Hself Hout Houtco Hrep.
 
+  (* Hypothesis STEPS: *)
+  (*   forall c (e: Clight.env), *)
+  (*     In c prog -> *)
+  (*     exists loc_f f, *)
+  (*       Globalenvs.Genv.find_symbol tge.(Clight.genv_genv) (step_id c.(c_name)) = Some loc_f *)
+  (*       /\ Maps.PTree.get (step_id c.(c_name)) e = None *)
+  (*       /\ Globalenvs.Genv.find_funct_ptr tge.(Clight.genv_genv) loc_f = Some (Ctypes.Internal f) *)
+  (*       /\ Clight.type_of_fundef (Ctypes.Internal f) = *)
+  (*         Ctypes.Tfunction (Ctypes.Tcons (type_of_inst_p c.(c_name)) *)
+  (*                                        (list_type_to_typelist (map snd (nelist2list c.(c_input) ++ nelist2list c.(c_output))))) *)
+  (*                                        Ctypes.Tvoid AST.cc_default *)
+  (*       /\ Coqlib.list_norepet (Clight.var_names (Clight.fn_params f) ++ Clight.var_names (Clight.fn_vars f)) *)
+  (*       /\ Clight.fn_body f = snd (translate_stmt c.(c_name) c.(c_step)) *)
+  (*       /\ length f.(Clight.fn_params) = 1 + Nelist.length c.(c_input)   *)
+  (*       /\ Forall (fun x => Ctypes.access_mode (snd x) = Ctypes.By_value (chunk_of_type (snd x))) *)
+  (*                (f.(Clight.fn_params) ++ f.(Clight.fn_vars)). *)
+  
+  Check stmt_eval_call_ind.
+  Theorem correctness:
+    (forall p S1 s S2,
+        stmt_eval p S1 s S2 ->
+        sub_prog p prog ->
+        forall c prog' f
+          (WF: well_formed_stmt c f s)
+          (Find: find_class c.(c_name) prog = Some (c, prog'))
+          (Hf: In f c.(c_methods)),
+        forall e1 le1 m1
+          (MS: match_states c f S1 (e1, le1, m1)),
+        exists le2 m2 T,
+          exec_stmt tge (function_entry2 tge) e1 le1 m1
+                    (translate_stmt prog c f s) T le2 m2 Out_normal
+          /\ match_states c f S2 (e1, le2, m2))
+    /\
+    (forall p me1 clsid fid vs me2 rvs,
+        stmt_call_eval p me1 clsid fid vs me2 rvs ->
+        sub_prog p prog ->
+        forall c caller S e1 le1 m1 o self out f ptr_f,
+          match_states c caller S (e1, le1, m1) ->
+          Globalenvs.Genv.find_symbol tge fid = Some ptr_f ->
+          Globalenvs.Genv.find_funct_ptr tge ptr_f = Some (Ctypes.Internal f) ->
+          find_inst S o me1 ->
+          exists m2 T,
+            eval_funcall tge (function_entry2 tge) m1 (Internal f)
+                         (self :: out :: vs) T m2 Vundef
+            /\ match_states c caller (update_inst S o me2) (e1, le1, m2)).
+  Proof.
+    clear TRANSL main_node_exists.
+    apply stmt_eval_call_ind;
+      [| |introv ? ? ? ? Hifte|introv ? HS1 ? HS2|introv ? Evs ? Hrec_eval|
+       |];
+      intros;
+      try inversion_clear WF as [? ? Hvars|? ? Hin| | |? ? ? ? ? ? ? ? ? Find' Findmeth|];
+      try (pose proof MS as MS'; inverts MS' as Hself Hout Houtco Hrep).
+    
     (* Assign x e : "x = e" *)
     - simpl; unfold assign.
       destruct (existsb (fun out => ident_eqb (fst out) x) f.(m_out)) eqn: E.
@@ -785,112 +851,85 @@ Section PRESERVATION.
         * simpl; apply* exp_eval_access.
         * unfold Int.add.
           rewrite* Int.unsigned_repr.
-          admit.
       
     (* Ifte e s1 s2 : "if e then s1 else s2" *)
-    - edestruct IHEV; destruct_conjs; eauto; [destruct* b|]. 
+    - edestruct Hifte; destruct_conjs; eauto; [destruct* b|]. 
       do 3 econstructor; split*.
       apply* exec_Sifthenelse.
       + erewrite type_pres, bool_val_ptr; eauto.
       + destruct* b.
       
     (* Comp s1 s2 : "s1; s2" *)
-    - app_stmt_eval_det.
-      edestruct IHEV1; destruct_conjs; eauto.
-      edestruct IHEV2; destruct_conjs; eauto.
+    - edestruct HS1; destruct_conjs; eauto.
+      edestruct HS2; destruct_conjs; eauto.
       do 3 econstructor; split*.
       apply* exec_Sseq_1.
       
     (* Step_ap y ty clsid o [e1; ... ;en] : "y = clsid_step(&(self->o), e1, ..., en)" *)
-    - do 3 econstructor; split.
+    - (* get the Clight corresponding function *)
+      forwards* Hin': find_class_In Find'.
+      (* pose proof Hstep as Hstep'. *)
+      (* edestruct Hstep' as (loc_f & f & ? & ? & ? & Htype_fun & ? & ? & Hlengths & ?); eauto. *)
+      (* rewrite <-type_pres' with (c:=c) (es:=es) (ys:=ys) in Htype_fun; auto. *)
+      forwards Eq: find_class_name Find'.
+      (* rewrite Eq in *; clear Eq. *)
+      
+      (* get the Clight corresponding field *)
+      (* pose proof Hself as Hself'. *)
+      (* destruct* Hself' as (? & ? & ? & ? & ? & ? & ? & ? & Hobj). *)
+      (* specializes Hobj Hin; destruct Hobj. *)
+
+      (* get outs values *)
+      (* edestruct exprlist_make_out_arg with (le:=le1) (c:=c) as (outs); eauto. *)
+      
+      (* recursive funcall evaluation *)
+      edestruct Hrec_eval with (c:=c) (e1:=e1) (m1:=m1) (le1:=le1) as (m2 & T & ? & ?); eauto.
+      skip.                     (* f ∈ tge *)
+      skip.                     (* f points to the function *)
+      exists le1 m2; econstructor; split.
       + simpl.
         unfold binded_funcall.
         rewrite Find', Findmeth.
         apply* exec_Sseq_1.
-        *{ eapply exec_Scall.
-           - simpl.
-             skip.
+        *{ eapply exec_Scall; eauto.
+           - reflexivity.
            - simpl.
              eapply eval_Elvalue.
              + apply eval_Evar_global.
-               * admit.
-               * skip.
+               * skip.          (* f ∉ e₁ *)
+               * skip.          (* f ∈ tge *)
              + apply* deref_loc_reference.               
            - apply find_method_In in Findmeth.
              econstructor.
              + eapply Clight.eval_Eaddrof. 
-               skip.
+               skip.            (* left-evaluation of self->o *)
              + eapply sem_cast_same. 
                unfold valid_val; splits*.
                * discriminate. 
                * simpl; trivial.
              + econstructor.
                * eapply Clight.eval_Eaddrof. 
-                 skip.
+                 skip.          (* left-evaluation of the out structure o *)
                *{ eapply sem_cast_same. 
                   unfold valid_val; splits*.
                   - discriminate. 
                   - simpl; trivial.
                 }
                * applys* exprs_eval_simu Find.
-           - skip.
-           - skip.
-           - skip.
+           - skip.              (* f points to the function *)
+           - skip.              (* type of the function *)
          }
-        * skip.
+        * simpl.
+          skip.                 (* ouput assignments *)
       + skip.
-      (* app_exps_eval_det. *)
-      (* app_find_inst_det. *)
-      (* app_stmt_step_eval_det'. *)
-      
-      (* (* get the Clight corresponding function *) *)
-      (* forwards* Hin': find_class_In Hfind. *)
-      (* pose proof Hstep as Hstep'. *)
-      (* edestruct Hstep' as (loc_f & f & ? & ? & ? & Htype_fun & ? & ? & Hlengths & ?); eauto. *)
-      (* rewrite <-type_pres' with (c:=c) (es:=es) (ys:=ys) in Htype_fun; auto. *)
-      (* forwards Eq: find_class_name Hfind. *)
-      (* rewrite Eq in *; clear Eq. *)
-      
-      (* (* get the Clight corresponding field *) *)
-      (* pose proof Hself as Hself'. *)
-      (* destruct* Hself' as (? & ? & ? & ? & ? & ? & ? & ? & Hobj). *)
-      (* specializes Hobj Hin; destruct Hobj.  *)
-
-      (* (* get outs values *) *)
-      (* edestruct exprlist_make_out_arg with (le:=le1) (c:=c) as (outs); eauto. *)
-      
-      (* (* recursive funcall evaluation *) *)
-      (* edestruct Hrec_eval with (c:=c) (e:=e1) (m:=m1) (le:=le1) (outs:=outs); destruct_conjs; eauto. *)
-      (* + rewrite <-ne_Forall2_lengths with (1:=Evs). *)
-      (*   rewrite Hlengths; simpl; f_equal. *)
-      (*   rewrite app_length; do 2 rewrite <-nelist2list_length. *)
-      (*   f_equal; symmetry; apply* ne_Forall2_lengths.         *)
-      (* + apply Clight.eval_Eaddrof; apply* evall_self_field. *)
-      (* + do 3 econstructor; split*. *)
-      (*   *{ apply* exec_Scall. *)
-      (*      - simpl; eauto. *)
-      (*      - eapply Clight.eval_Elvalue. *)
-      (*        + apply* Clight.eval_Evar_global. *)
-      (*        + apply* Clight.deref_loc_reference. *)
-      (*      - econstructor. *)
-      (*        + eapply Clight.eval_Eaddrof. *)
-      (*          apply* evall_self_field. *)
-      (*        + eapply sem_cast_same. *)
-      (*          unfold valid_val; splits*. *)
-      (*          * discriminate. *)
-      (*          * simpl; trivial. *)
-      (*        + apply* eval_exprlist_app. *)
-      (*          apply* exprs_eval_simu. *)
-      (*      - eauto. *)
-      (*    } *)
-      (*   * admit.  *)
       
     (* Skip : "skip" *)
     - do 3 econstructor; split*.
       eapply exec_Sskip.
 
     (* funcall *)
-    (* - (* forwards* Hfind'': find_class_sub_same Hfind UNIQUE. *) *)
+    - admit.
+      (* forwards* Hfind'': find_class_sub_same Hfind UNIQUE. *)
       (* rewrite Hfind' in Hfind''; inverts Hfind''. *)
       (* destruct Hstep with (c:=cls) *)
       (*   as (loc_f' & f' & Hget_loc_f' & Hget_f' & Htype_fun & Hvars_nil & ? & ? & Htr & ?); *)
@@ -934,775 +973,3 @@ Section PRESERVATION.
       (*   * admit. *)
       (*   * admit. *)
   Qed.
-  
-  
-  (* Definition nodup_env (e: Clight.env) := *)
-  (*   forall x x' loc t t', *)
-  (*     x' <> x -> *)
-  (*     Maps.PTree.get x e = Some (loc, t) -> *)
-  (*     Maps.PTree.get x' e <> Some (loc, t'). *)
-
-  (* Definition nodup_fields (co: Ctypes.composite) := *)
-  (*   forall x t t', *)
-  (*     In (x, t) (Ctypes.co_members co) -> *)
-  (*     In (x, t') (Ctypes.co_members co) -> *)
-  (*     t' = t. *)
-
-  (* Definition nodup_vars (c: class) := *)
-  (*   forall x t t', *)
-  (*     In (x, t) (class_vars c) -> *)
-  (*     In (x, t') (class_vars c) -> *)
-  (*     t' = t. *)
-
-  (*  Definition nodup_mems (c: class) := *)
-  (*   forall x t t', *)
-  (*     In (x, t) c.(c_mems) -> *)
-  (*     In (x, t') c.(c_mems) -> *)
-  (*     t' = t. *)
-  
-  (* Remark find_add: *)
-  (*   forall x (v v': val) pm,  *)
-  (*     PM.find x (PM.add x v pm) = Some v' -> v' = v. *)
-  (* Proof. *)
-  (*   induction x, pm; simpl; (eauto || now injection 1). *)
-  (* Qed. *)
-
-  (* Remark find_update_var: *)
-  (*   forall x v v' S, *)
-  (*     find_var (update_var S x v) x v' -> v' = v. *)
-  (* Proof. *)
-  (*   unfold find_var, update_var; simpl. *)
-  (*   intros; apply* find_add. *)
-  (* Qed. *)
-
-  (* Remark find_update_field: *)
-  (*   forall x v v' S, *)
-  (*     find_field (update_field S x v) x v' -> v' = v. *)
-  (* Proof. *)
-  (*   unfold find_field, update_field, mfind_mem, madd_mem; simpl. *)
-  (*   intros; apply* find_add. *)
-  (* Qed. *)
-
-  (* Remark gso_var: *)
-  (*   forall x x' v v' S, *)
-  (*     x <> x' -> find_var (update_var S x' v) x v' -> find_var S x v'. *)
-  (* Proof. *)
-  (*   unfold find_var, update_var; simpl. *)
-  (*   introv Neq H. *)
-  (*   rewrite <-H; symmetry. *)
-  (*   apply* PM.gso. *)
-  (* Qed. *)
-
-  (* Remark gso_field: *)
-  (*   forall x x' v v' S, *)
-  (*     x <> x' -> find_field (update_field S x' v) x v' -> find_field S x v'. *)
-  (* Proof. *)
-  (*   unfold find_field, update_field; simpl. *)
-  (*   introv Neq H. *)
-  (*   rewrite <-H; symmetry. *)
-  (*   apply* mfind_mem_gso. *)
-  (* Qed. *)
-
-  (* Remark find_field_update_var: *)
-  (*   forall S x v x' v', *)
-  (*     find_field (update_var S x v) x' v' -> find_field S x' v'. *)
-  (* Proof. unfold find_field, update_var; simpl; auto. Qed. *)
-
-  (* Remark find_var_update_field: *)
-  (*   forall S x v x' v', *)
-  (*     find_var (update_field S x v) x' v' -> find_var S x' v'. *)
-  (* Proof. unfold find_var, update_field; simpl; auto. Qed. *)
-
-  (* Definition mem_sep (c: class) (e: Clight.env) (m: Memory.Mem.mem) := *)
-  (*   forall x loc t loc_self loc_struct ofs, *)
-  (*     In (x, t) (class_vars c) ->  *)
-  (*     Maps.PTree.get x e = Some (loc, t) -> *)
-  (*     Maps.PTree.get self_id e = Some (loc_self, pointer_of_node c.(c_name)) -> *)
-  (*     Memory.Mem.load AST.Mint32 m loc_self 0 = Some (Values.Vptr loc_struct ofs) -> *)
-  (*     loc <> loc_struct. *)
-
-  (* Definition self_sep (c: class) (e: Clight.env) (m: Memory.Mem.mem) := *)
-  (*   forall loc_self loc_struct ofs, *)
-  (*     Maps.PTree.get self_id e = Some (loc_self, pointer_of_node c.(c_name)) -> *)
-  (*     Memory.Mem.load AST.Mint32 m loc_self 0 = Some (Values.Vptr loc_struct ofs) -> *)
-  (*     loc_struct <> loc_self. *)
-
-  (* Definition fields_sep (m: Memory.Mem.mem) := *)
-  (*   forall co x x' t t' ofs delta delta', *)
-  (*     x <> x' -> *)
-  (*     Ctypes.field_offset (Clight.genv_cenv tge) x (Ctypes.co_members co) = Errors.OK delta -> *)
-  (*     Ctypes.field_offset (Clight.genv_cenv tge) x' (Ctypes.co_members co) = Errors.OK delta' -> *)
-  (*     (BinInt.Z.le *)
-  (*        (BinInt.Z.add (Int.unsigned (Int.add ofs (Int.repr delta'))) *)
-  (*                      (Memdata.size_chunk (chunk_of_type t'))) *)
-  (*        (Int.unsigned (Int.add ofs (Int.repr delta))) *)
-  (*      \/ *)
-  (*      BinInt.Z.le *)
-  (*        (BinInt.Z.add (Int.unsigned (Int.add ofs (Int.repr delta))) *)
-  (*                      (Memdata.size_chunk (chunk_of_type t))) *)
-  (*        (Int.unsigned (Int.add ofs (Int.repr delta')))). *)
-
-  (* (* Hypothesis STEPS: *) *)
-  (* (*   forall c (e: Clight.env), *) *)
-  (* (*     In c prog -> *) *)
-  (* (*     exists loc_f f, *) *)
-  (* (*       Globalenvs.Genv.find_symbol tge.(Clight.genv_genv) (step_id c.(c_name)) = Some loc_f *) *)
-  (* (*       /\ Maps.PTree.get (step_id c.(c_name)) e = None *) *)
-  (* (*       /\ Globalenvs.Genv.find_funct_ptr tge.(Clight.genv_genv) loc_f = Some (Ctypes.Internal f) *) *)
-  (* (*       /\ Clight.type_of_fundef (Ctypes.Internal f) = *) *)
-  (* (*         Ctypes.Tfunction (Ctypes.Tcons (type_of_inst_p c.(c_name)) *) *)
-  (* (*                                        (list_type_to_typelist (map snd (nelist2list c.(c_input) ++ nelist2list c.(c_output))))) *) *)
-  (* (*                                        Ctypes.Tvoid AST.cc_default *) *)
-  (* (*       /\ Coqlib.list_norepet (Clight.var_names (Clight.fn_params f) ++ Clight.var_names (Clight.fn_vars f)) *) *)
-  (* (*       /\ Clight.fn_body f = snd (translate_stmt c.(c_name) c.(c_step)) *) *)
-  (* (*       /\ length f.(Clight.fn_params) = 1 + Nelist.length c.(c_input)   *) *)
-  (* (*       /\ Forall (fun x => Ctypes.access_mode (snd x) = Ctypes.By_value (chunk_of_type (snd x))) *) *)
-  (* (*                (f.(Clight.fn_params) ++ f.(Clight.fn_vars)). *) *)
-  
-  (* Definition match_step (e: Clight.env) := *)
-  (*   forall c, *)
-  (*     In c prog -> *)
-  (*     exists loc_f f, *)
-  (*       Globalenvs.Genv.find_symbol tge.(Clight.genv_genv) (step_id c.(c_name)) = Some loc_f *)
-  (*       /\ Maps.PTree.get (step_id c.(c_name)) e = None *)
-  (*       /\ Globalenvs.Genv.find_funct_ptr tge.(Clight.genv_genv) loc_f = Some (Ctypes.Internal f) *)
-  (*       /\ Clight.type_of_fundef (Ctypes.Internal f) = *)
-  (*         Ctypes.Tfunction (Ctypes.Tcons (type_of_inst_p c.(c_name)) *)
-  (*                                        (list_type_to_typelist *)
-  (*                                           (map snd (nelist2list c.(c_input) ++ nelist2list c.(c_output))))) *)
-  (*                          Ctypes.Tvoid AST.cc_default *)
-  (*       (* /\ f.(Clight.fn_vars) = [] *) *)
-  (*       /\ Coqlib.list_norepet (Clight.var_names (Clight.fn_params f) ++ Clight.var_names (Clight.fn_vars f)) *)
-  (*       /\ Clight.fn_body f = Clight.Ssequence (translate_stmt c.(c_name) c.(c_step)) (Clight.Sreturn None) *)
-  (*       /\ f.(Clight.fn_params) = *)
-  (*         (self_id, type_of_inst_p c.(c_name)) :: nelist2list c.(c_input) ++ nelist2list c.(c_output) *)
-  (*       /\ Forall (fun x => Ctypes.access_mode (snd x) = Ctypes.By_value (chunk_of_type (snd x))) *)
-  (*                (f.(Clight.fn_params) ++ f.(Clight.fn_vars)). *)
-  
-  (* Definition c_state := (Clight.env * Memory.Mem.mem)%type. *)
-   
-  (* Inductive match_states (c: class) (S: state): c_state -> Prop := *)
-  (*   intro_match_states: forall e m, *)
-  (*     (* state correspondance *) *)
-  (*     compat_vars c S e m -> *)
-  (*     compat_self c S e m -> *)
-
-  (*     (* function *) *)
-  (*     match_step e -> *)
-      
-  (*     (* Clight side separation *) *)
-  (*     mem_sep c e m -> *)
-  (*     self_sep c e m -> *)
-  (*     fields_sep m -> *)
-  (*     nodup_env e -> *)
-
-  (*     (* Minimp side separation *) *)
-  (*     nodup_vars c -> *)
-  (*     nodup_mems c -> *)
-  (*     match_states c S (e, m). *)
-
-  (* Hint Constructors match_states. *)
-  
-  (* Remark load_same: *)
-  (*   forall env x t x' t' m m' chk loc loc' v vptr vptr', *)
-  (*     nodup_env env -> *)
-  (*     x <> x' -> *)
-  (*     Maps.PTree.get x env = Some (loc, t) -> *)
-  (*     Maps.PTree.get x' env = Some (loc', t') -> *)
-  (*     Memory.Mem.store chk m loc 0 v = Some m' -> *)
-  (*     Memory.Mem.load AST.Mint32 m loc' 0 = Some vptr -> *)
-  (*     Memory.Mem.load AST.Mint32 m' loc' 0 = Some vptr' -> *)
-  (*     vptr' = vptr. *)
-  (* Proof. *)
-  (*   introv Hnodupenv ? ? ? ? Hload Hload'. *)
-  (*   destruct (Values.eq_block loc loc'). *)
-  (*     + subst loc. *)
-  (*       edestruct Hnodupenv; eauto. *)
-  (*     + assert (Memory.Mem.load AST.Mint32 m' loc' 0 = Memory.Mem.load AST.Mint32 m loc' 0) *)
-  (*         as Eq by apply* Memory.Mem.load_store_other. *)
-  (*       rewrite Eq in Hload'; rewrite Hload' in Hload; inverts Hload. *)
-  (*       reflexivity.         *)
-  (* Qed. *)
-  
-  (* Lemma compat_assign_pres: *)
-  (*   forall c S e m loc x t v, *)
-  (*     In c prog -> *)
-  (*     match_states c S (e, m) -> *)
-  (*     Maps.PTree.get x e = Some (loc, t) -> *)
-  (*     In (x, t) (class_vars c) -> *)
-  (*     v = Values.Val.load_result (chunk_of_type t) v -> *)
-  (*     valid_val v t -> *)
-  (*     x <> self_id -> *)
-  (*     exists m', Memory.Mem.store (chunk_of_type t) m loc 0 v = Some m'  *)
-  (*           /\ match_states c (update_var S x v) (e, m'). *)
-  (* Proof. *)
-  (*   introv ? MS Hget Hin Hloadres ? ?. *)
-  (*   inverts MS as Hvars Hself Hstep Hsep Hself_sep Hfields_sep Hnodupenv Hnodupvars; intro Hnodupmems. *)
-  (*   edestruct Hvars as (loc' & Hget' & ? & ?); eauto. *)
-  (*   rewrite Hget' in Hget; inverts Hget; rename Hget' into Hget. *)
-  (*   edestruct Memory.Mem.valid_access_store with (v:=v) as [m']; eauto. *)
-  (*   destruct* Hself as (co & loc_self & loc_struct & ofs & Hget_self & Hload_self & Hget_co & Hmem & ?). *)
-  (*   exists m'; split*; constructor*. *)
-
-  (*   - unfold compat_vars; intros x' t' ? Hin'. *)
-  (*     edestruct Hvars as (loc' & Hget' & ? & Hm); eauto. *)
-  (*     exists loc'; splits*. *)
-  (*     + apply* Memory.Mem.store_valid_access_1. *)
-  (*     + intros v' Hfind. *)
-  (*       destruct (AST.ident_eq x' x). *)
-  (*       *{ subst x'. *)
-  (*          apply find_update_var in Hfind; subst v'. *)
-  (*          specializes Hnodupvars Hin Hin'; subst t'.  *)
-  (*          split*. *)
-  (*          destruct (Values.eq_block loc' loc) as [|Neq]. *)
-  (*          - subst loc'. *)
-  (*            rewrite Hloadres; apply* Memory.Mem.load_store_same. *)
-  (*          - rewrite Hget in Hget'; inverts Hget'. now contradict Neq.  *)
-  (*        } *)
-  (*       *{ apply gso_var in Hfind; auto. *)
-  (*          forwards (Hload & ?): Hm Hfind.  *)
-  (*          split*. *)
-  (*          destruct (Values.eq_block loc' loc). *)
-  (*          - subst loc'. *)
-  (*            edestruct Hnodupenv; eauto.  *)
-  (*          - rewrite <-Hload.  *)
-  (*            apply* Memory.Mem.load_store_other. *)
-  (*        }         *)
-         
-  (*   - unfold compat_self; intro. *)
-  (*     exists co loc_self loc_struct ofs. *)
-  (*     splits*. *)
-  (*     + destruct (Values.eq_block loc_self loc). *)
-  (*       * subst loc. *)
-  (*         edestruct Hnodupenv; eauto. *)
-  (*       * rewrite <-Hload_self. *)
-  (*         apply* Memory.Mem.load_store_other. *)
-  (*     + intros x' t' Hin'. *)
-  (*       specializes Hmem Hin'; destruct Hmem as (delta & ? & ? & ? & Hm). *)
-  (*       exists delta; splits*. *)
-  (*        * apply* Memory.Mem.store_valid_access_1. *)
-  (*        *{ intros v' Hfind. *)
-  (*           apply find_field_update_var in Hfind. *)
-  (*           forwards (Hload & ?): Hm Hfind. *)
-  (*           splits*. *)
-  (*           destruct (Values.eq_block loc loc_struct). *)
-  (*           - edestruct Hsep; eauto. *)
-  (*           - rewrite <-Hload. *)
-  (*             apply* Memory.Mem.load_store_other. *)
-  (*         } *)
-
-  (*   - unfold mem_sep; introv ? ? Hget_self' ?. *)
-  (*     rewrite Hget_self' in Hget_self; inverts Hget_self. *)
-  (*     forwards* Eq: load_same; inverts Eq. *)
-  (*     apply* Hsep. *)
-
-  (*   - unfold self_sep; introv Hget_self' ?. *)
-  (*     rewrite Hget_self' in Hget_self; inverts Hget_self. *)
-  (*     forwards* Eq: load_same; inverts Eq. *)
-  (*     apply* Hself_sep. *)
-  (* Qed. *)
-
-  (* (* Lemma compat_assigns_pres: *) *)
-  (* (*   forall c S e m loc ys vs, *) *)
-  (* (*     In c prog -> *) *)
-  (* (*     match_states c S (e, m) -> *) *)
-  (* (*     Nelist.Forall (fun y => In y (class_vars c)) ys -> *) *)
-  (* (*     exists m', Memory.Mem.store (chunk_of_type t) m loc 0 v = Some m'  *) *)
-  (* (*           /\ match_states c (update_var S x v) (e, m'). *) *)
-  (* (* Proof. *) *)
-  (* (*   introv ? MS Hget Hin Hloadres ? ?. *) *)
-  (* (*   inverts MS as Hvars Hself Hstep Hsep Hself_sep Hfields_sep Hnodupenv Hnodupvars; intro Hnodupmems. *) *)
-  (* (*   edestruct Hvars as (loc' & Hget' & ? & ?); eauto. *) *)
-  (* (*   rewrite Hget' in Hget; inverts Hget; rename Hget' into Hget. *) *)
-  (* (*   edestruct Memory.Mem.valid_access_store with (v:=v) as [m']; eauto. *) *)
-  (* (*   destruct* Hself as (co & loc_self & loc_struct & ofs & Hget_self & Hload_self & Hget_co & Hmem & ?). *) *)
-  (* (*   exists m'; split*; constructor*. *) *)
-
-  (* (*   - unfold compat_vars; intros x' t' ? Hin'. *) *)
-  (* (*     edestruct Hvars as (loc' & Hget' & ? & Hm); eauto. *) *)
-  (* (*     exists loc'; splits*. *) *)
-  (* (*     + apply* Memory.Mem.store_valid_access_1. *) *)
-  (* (*     + intros v' Hfind. *) *)
-  (* (*       destruct (AST.ident_eq x' x). *) *)
-  (* (*       *{ subst x'. *) *)
-  (* (*          apply find_update_var in Hfind; subst v'. *) *)
-  (* (*          specializes Hnodupvars Hin Hin'; subst t'.  *) *)
-  (* (*          split*. *) *)
-  (* (*          destruct (Values.eq_block loc' loc) as [|Neq]. *) *)
-  (* (*          - subst loc'. *) *)
-  (* (*            rewrite Hloadres; apply* Memory.Mem.load_store_same. *) *)
-  (* (*          - rewrite Hget in Hget'; inverts Hget'. now contradict Neq.  *) *)
-  (* (*        } *) *)
-  (* (*       *{ apply gso_var in Hfind; auto. *) *)
-  (* (*          forwards (Hload & ?): Hm Hfind.  *) *)
-  (* (*          split*. *) *)
-  (* (*          destruct (Values.eq_block loc' loc). *) *)
-  (* (*          - subst loc'. *) *)
-  (* (*            edestruct Hnodupenv; eauto.  *) *)
-  (* (*          - rewrite <-Hload.  *) *)
-  (* (*            apply* Memory.Mem.load_store_other. *) *)
-  (* (*        }         *) *)
-         
-  (* (*   - unfold compat_self; intro. *) *)
-  (* (*     exists co loc_self loc_struct ofs. *) *)
-  (* (*     splits*. *) *)
-  (* (*     + destruct (Values.eq_block loc_self loc). *) *)
-  (* (*       * subst loc. *) *)
-  (* (*         edestruct Hnodupenv; eauto. *) *)
-  (* (*       * rewrite <-Hload_self. *) *)
-  (* (*         apply* Memory.Mem.load_store_other. *) *)
-  (* (*     + intros x' t' Hin'. *) *)
-  (* (*       specializes Hmem Hin'; destruct Hmem as (delta & ? & ? & ? & Hm). *) *)
-  (* (*       exists delta; splits*. *) *)
-  (* (*        * apply* Memory.Mem.store_valid_access_1. *) *)
-  (* (*        *{ intros v' Hfind. *) *)
-  (* (*           apply find_field_update_var in Hfind. *) *)
-  (* (*           forwards (Hload & ?): Hm Hfind. *) *)
-  (* (*           splits*. *) *)
-  (* (*           destruct (Values.eq_block loc loc_struct). *) *)
-  (* (*           - edestruct Hsep; eauto. *) *)
-  (* (*           - rewrite <-Hload. *) *)
-  (* (*             apply* Memory.Mem.load_store_other. *) *)
-  (* (*         } *) *)
-
-  (* (*   - unfold mem_sep; introv ? ? Hget_self' ?. *) *)
-  (* (*     rewrite Hget_self' in Hget_self; inverts Hget_self. *) *)
-  (* (*     forwards* Eq: load_same; inverts Eq. *) *)
-  (* (*     apply* Hsep. *) *)
-
-  (* (*   - unfold self_sep; introv Hget_self' ?. *) *)
-  (* (*     rewrite Hget_self' in Hget_self; inverts Hget_self. *) *)
-  (* (*     forwards* Eq: load_same; inverts Eq. *) *)
-  (* (*     apply* Hself_sep. *) *)
-  (* (* Qed. *) *)
-
-  (* Remark load_same': *)
-  (*   forall c env m m' chk loc' v ofs loc1 ofs1 loc2 ofs2, *)
-  (*     self_sep c env m -> *)
-  (*     Maps.PTree.get self_id env = Some (loc', pointer_of_node c.(c_name)) -> *)
-  (*     Memory.Mem.store chk m loc1 ofs v = Some m' -> *)
-  (*     Memory.Mem.load AST.Mint32 m loc' 0 = Some (Values.Vptr loc1 ofs1) -> *)
-  (*     Memory.Mem.load AST.Mint32 m' loc' 0 = Some (Values.Vptr loc2 ofs2) -> *)
-  (*     Values.Vptr loc1 ofs1 = Values.Vptr loc2 ofs2. *)
-  (* Proof. *)
-  (*   introv Hself_sep ? ? Hload1 Hload2. *)
-  (*   assert (Memory.Mem.load AST.Mint32 m' loc' 0 = Memory.Mem.load AST.Mint32 m loc' 0) *)
-  (*     as Eq. *)
-  (*   apply* Memory.Mem.load_store_other. *)
-  (*   left; intro Eq; symmetry in Eq; revert Eq; apply* Hself_sep. *)
-  (*   rewrite Eq in Hload2; rewrite Hload2 in Hload1; inverts Hload1. *)
-  (*   reflexivity. *)
-  (* Qed. *)
-
-  (* Lemma compat_stassign_pres: *)
-  (*   forall c S e m x t v co loc_self loc_struct ofs delta, *)
-  (*     In c prog -> *)
-  (*     match_states c S (e, m) -> *)
-  (*     Ctypes.field_offset tge.(Clight.genv_cenv) x (Ctypes.co_members co) = Errors.OK delta -> *)
-  (*     Maps.PTree.get c.(c_name) (Clight.genv_cenv tge) = Some co -> *)
-  (*     Maps.PTree.get self_id e = Some (loc_self, pointer_of_node c.(c_name)) -> *)
-  (*     Memory.Mem.load AST.Mint32 m loc_self 0 = Some (Values.Vptr loc_struct ofs) -> *)
-  (*     In (x, t) c.(c_mems) -> *)
-  (*     v = Values.Val.load_result (chunk_of_type t) v -> *)
-  (*     valid_val v t -> *)
-  (*    Memory.Mem.valid_access m (chunk_of_type t) loc_struct (Int.unsigned (Int.add ofs (Int.repr delta))) Memtype.Writable -> *)
-  (*     exists m', *)
-  (*       Memory.Mem.store (chunk_of_type t) m loc_struct (Int.unsigned (Int.add ofs (Int.repr delta))) v = Some m' *)
-  (*       /\ match_states c (update_field S x v) (e, m'). *)
-  (* Proof. *)
-  (*   intros ** ? MS Hoffset Hget_co Hget_self Hload_self Hin Hloadres ? ? . *)
-  (*   inverts MS as Hvars Hself Hstep Hsep Hself_sep Hfields_sep Hnodupenv Hnodupvars; intro Hnodupmems. *)
-  (*   edestruct Memory.Mem.valid_access_store with (v:=v) as [m']; eauto.  *)
-  (*   exists m'; split*; constructor*. *)
-
-  (*   - unfold compat_vars; intros. *)
-  (*     edestruct Hvars as (loc & ? & ? & Hm); eauto. *)
-  (*     exists loc; splits*. *)
-  (*     + apply* Memory.Mem.store_valid_access_1. *)
-  (*     + introv Hfind. *)
-  (*       apply find_var_update_field in Hfind. *)
-  (*       forwards (Hload & ?): Hm Hfind. *)
-  (*       split*. *)
-  (*       destruct (Values.eq_block loc loc_struct). *)
-  (*       * edestruct Hsep; eauto. *)
-  (*       * rewrite <-Hload. *)
-  (*         apply* Memory.Mem.load_store_other. *)
-
-  (*   - unfold compat_self; intro. *)
-  (*     exists co loc_self loc_struct ofs. *)
-  (*     destruct* Hself as (? & ? & ? & ? & Hget_self' & Hload_self' & Hget_co' & Hmem & ?). *)
-  (*     rewrite Hget_co' in Hget_co; inverts Hget_co. *)
-  (*     rewrite Hget_self' in Hget_self; inverts Hget_self. *)
-  (*     rewrite Hload_self' in Hload_self; inverts Hload_self.   *)
-  (*     splits*. *)
-  (*     + destruct (Values.eq_block loc_self loc_struct). *)
-  (*       * edestruct Hself_sep; eauto. *)
-  (*       * rewrite <-Hload_self'. *)
-  (*         apply* Memory.Mem.load_store_other. *)
-  (*     + intros x' t' Hin'. *)
-  (*       specializes Hmem Hin'; destruct Hmem as (delta' & Hoffset' & ? & ? & Hm). *)
-  (*       exists delta'; splits*. *)
-  (*       * apply* Memory.Mem.store_valid_access_1.   *)
-  (*       *{ intros v' Hfind'. *)
-  (*          destruct (AST.ident_eq x' x). *)
-  (*          - subst x'. *)
-  (*            rewrite Hoffset' in Hoffset; inverts Hoffset. *)
-  (*            apply find_update_field in Hfind'; subst v'. *)
-  (*            specializes Hnodupmems Hin Hin'; subst t'.  *)
-  (*            split*. *)
-  (*            rewrite Hloadres; apply* Memory.Mem.load_store_same. *)
-  (*          - apply gso_field in Hfind'; auto. *)
-  (*            forwards (Hload & ?): Hm Hfind'. *)
-  (*            split*. *)
-  (*            rewrite <-Hload; apply* Memory.Mem.load_store_other. *)
-  (*        } *)
-        
-  (*   - unfold mem_sep; introv ? ? Hget_self' ?. *)
-  (*     rewrite Hget_self' in Hget_self; inverts Hget_self. *)
-  (*     forwards* Eq: load_same'; inverts Eq. *)
-  (*     apply* Hsep. *)
-
-  (*   - unfold self_sep; introv Hget_self' ?. *)
-  (*     rewrite Hget_self' in Hget_self; inverts Hget_self. *)
-  (*     forwards* Eq: load_same'; inverts Eq. *)
-  (*     apply* Hself_sep. *)
-  (* Qed. *)
-  
-  (* Remark alloc_exists: *)
-  (*   forall vars e m, *)
-  (*     exists e' m', *)
-  (*       Clight.alloc_variables tge e m vars e' m'. *)
-  (* Proof. *)
-  (*   induction vars as [|(x, ty)]. *)
-  (*   - do 3 econstructor. *)
-  (*   - intros. *)
-  (*     destruct (Memory.Mem.alloc m 0 (Ctypes.sizeof (Clight.genv_cenv tge) ty)) eqn: Eq. *)
-  (*     specialize (IHvars (Maps.PTree.set x (b, ty) e) m0). *)
-  (*     destruct* IHvars as (? & ? & ?). *)
-  (*     do 3 econstructor; eauto. *)
-  (* Qed. *)
-
-  (* Remark assign_loc_exists: *)
-  (*   forall v ty m loc, *)
-  (*     Ctypes.access_mode ty = Ctypes.By_value (chunk_of_type ty) -> *)
-  (*     Memory.Mem.valid_access m (chunk_of_type ty) loc 0 Memtype.Writable -> *)
-  (*     exists m', *)
-  (*       Clight.assign_loc tge.(Clight.genv_cenv) ty m loc Int.zero v m'. *)
-  (* Proof. *)
-  (*   introv ? Hvalid. *)
-  (*   forwards (? & ?): Memory.Mem.valid_access_store Hvalid. *)
-  (*   do 2 econstructor; eauto. *)
-  (* Qed. *)
-  
-  (* Remark bind_parameters_exists: *)
-  (*   forall xs vs e m, *)
-  (*     length xs = length vs -> *)
-  (*     Forall (fun x => exists loc, *)
-  (*                 Maps.PTree.get (fst x) e = Some (loc, snd x) *)
-  (*                 /\ Memory.Mem.valid_access m (chunk_of_type (snd x)) loc 0 Memtype.Writable *)
-  (*                 /\ Ctypes.access_mode (snd x) = Ctypes.By_value (chunk_of_type (snd x))) xs -> *)
-  (*     exists m', *)
-  (*       Clight.bind_parameters tge e m xs vs m'. *)
-  (* Proof. *)
-  (*   induction xs as [|(x, ty)]; destruct vs; introv Hlengths Hparams; try discriminate. *)
-  (*   - do 2 econstructor. *)
-  (*   - inverts Hparams as (? & ? & Hvalid & Haccess) Hparams.   *)
-  (*     forwards (m' & Hassign): (assign_loc_exists v) Haccess Hvalid. *)
-  (*     edestruct IHxs with (m:=m') (e:=e); eauto. *)
-  (*     + inversion_clear Hassign as [|? ? ? ? Haccess']. *)
-  (*       *{ clear IHxs Hlengths. induction xs. *)
-  (*          - constructor. *)
-  (*          - inverts Hparams as (loc & ?). *)
-  (*            constructor. *)
-  (*            + exists loc; splits*. *)
-  (*              apply* Memory.Mem.store_valid_access_1. *)
-  (*            + apply* IHxs. *)
-  (*        } *)
-  (*       * rewrite Haccess' in Haccess; discriminate. *)
-  (*     + do 2 econstructor; eauto.  *)
-  (* Qed. *)
-
-  (* Remark alloc_variables_implies: *)
-  (*   forall vars e m e' m',  *)
-  (*     Clight.alloc_variables tge e m vars e' m' -> *)
-  (*     Forall (fun x => Ctypes.access_mode (snd x) = Ctypes.By_value (chunk_of_type (snd x))) vars -> *)
-  (*     Forall (fun x => exists loc, *)
-  (*                 Maps.PTree.get (fst x) e' = Some (loc, snd x) *)
-  (*                 /\ Memory.Mem.valid_access m' (chunk_of_type (snd x)) loc 0 Memtype.Writable *)
-  (*                 /\ Ctypes.access_mode (snd x) = Ctypes.By_value (chunk_of_type (snd x))) vars. *)
-  (* Proof. *)
-  (*   induction vars. *)
-  (*   - constructor. *)
-  (*   - introv Halloc Hforall. *)
-  (*     inverts Halloc. *)
-  (*     constructor. *)
-  (*     + exists b1; splits*. *)
-  (*       * admit. *)
-  (*       *{ assert (Memory.Mem.valid_access m1 (chunk_of_type (snd (id, ty))) b1 0 Memtype.Writable). *)
-  (*          - eapply Memory.Mem.valid_access_freeable_any. *)
-  (*            apply* Memory.Mem.valid_access_alloc_same. *)
-  (*            + omega. *)
-  (*            + simpl. admit. *)
-  (*            + eapply BinInt.Z.divide_0_r. *)
-  (*          - admit. *)
-  (*        } *)
-  (*       * inverts* Hforall. *)
-  (*     + apply* IHvars. *)
-  (*       inverts* Hforall. *)
-  (* Qed. *)
-
-  (* Remark forall_app: *)
-  (*   forall A (P: A -> Prop) l1 l2, *)
-  (*     Forall P (l1 ++ l2) -> Forall P l1 /\ Forall P l2. *)
-  (* Proof. *)
-  (*   introv HForall; split; rewrite Forall_forall in *; introv Hin; *)
-  (*   apply HForall; apply in_or_app; [left | right]; auto. *)
-  (* Qed. *)
-
-  (* Lemma compat_funcall_pres: *)
-  (*   forall m f vargs, *)
-  (*     Datatypes.length (Clight.fn_params f) = Datatypes.length vargs -> *)
-  (*     Forall (fun x => Ctypes.access_mode (snd x) = Ctypes.By_value (chunk_of_type (snd x))) (f.(Clight.fn_params) ++ f.(Clight.fn_vars)) -> *)
-  (*     exists m1 e_fun m2, *)
-  (*       Clight.alloc_variables tge Clight.empty_env m (f.(Clight.fn_params) ++ f.(Clight.fn_vars)) e_fun m1  *)
-  (*       /\ Clight.bind_parameters tge e_fun m1 f.(Clight.fn_params) vargs m2. *)
-  (* Proof. *)
-  (*   introv Hlengths Haccesses. *)
-  (*   forwards (e_fun & m1 & Halloc): *)
-  (*     (alloc_exists (f.(Clight.fn_params) ++ f.(Clight.fn_vars)) Clight.empty_env m). *)
-  (*   exists m1 e_fun. *)
-  (*   forwards* Hforall': alloc_variables_implies Halloc Haccesses. *)
-  (*   forwards (Hforall & H'): forall_app Hforall'; clear Hforall' H'. *)
-  (*   forwards* (m2 & ?): bind_parameters_exists Hlengths Hforall. *)
-  (* Qed. *)
-  
-  (* Remark type_pres': *)
-  (*   forall c' c es ys, *)
-  (*     Nelist.Forall2 (fun e x => typeof e = snd x) es c'.(c_input) -> *)
-  (*     map Clight.typeof (nelist2list (Nelist.map (translate_exp c.(c_name)) es) *)
-  (*                        ++ nelist2list (Nelist.map make_out_arg ys)) = *)
-  (*     map snd (nelist2list c'.(c_input) ++ nelist2list c'.(c_output)). *)
-  (* Proof. *)
-  (*   (* intros c'. *) *)
-  (*   (* induction (c_input c'); introv Heq; *) *)
-  (*   (* inversion_clear Heq as [? ? Hty|? ? ? ? Hty Hforall2]; simpl. *) *)
-  (*   (* - rewrite type_pres, Hty; auto. *) *)
-  (*   (* - f_equal. *) *)
-  (*   (*   + rewrite type_pres, Hty; auto. *) *)
-  (*   (*   + specializes IHn Hforall2; eauto. *) *)
-  (*   admit. *)
-  (* Qed. *)
-
-  (* Hint Constructors Clight.eval_lvalue Clight.eval_expr well_formed_stmt. *)
-  (* Hint Resolve expr_eval_simu Clight.assign_loc_value sem_cast_same. *)
-  (* Hint Constructors well_formed_stmt. *)
-
-  (* Remark ne_Forall2_lengths: *)
-  (*   forall A B (P: A -> B -> Prop) l1 l2, *)
-  (*     Nelist.Forall2 P l1 l2 -> Nelist.length l1 = Nelist.length l2. *)
-  (* Proof. *)
-  (*   induction l1, l2; introv HForall2; inverts* HForall2. *)
-  (*   simpl; f_equal; apply* IHl1. *)
-  (* Qed. *)
-
-  (* Lemma exprlist_make_out_arg: *)
-  (*   forall c S e le m ys, *)
-  (*     In c prog -> *)
-  (*     compat_vars c S e m -> *)
-  (*     Nelist.Forall (fun y => In y (class_vars c)) ys -> *)
-  (*     exists vs, Clight.eval_exprlist tge e le m *)
-  (*                                (nelist2list (Nelist.map make_out_arg ys)) *)
-  (*                                (list_type_to_typelist *)
-  (*                                   (map Clight.typeof (nelist2list (Nelist.map make_out_arg ys)))) *)
-  (*                                vs. *)
-  (* Proof. *)
-  (*   introv ? Hvars Hins. *)
-  (*   induction ys as [[x t]|[x t]]; inverts Hins as ? Hins; *)
-  (*   edestruct Hvars; eauto. *)
-  (*   - do 2 econstructor; eauto. *)
-  (*     + apply Clight.eval_Eaddrof. *)
-  (*       apply* Clight.eval_Evar_local. *)
-  (*     + apply sem_cast_same. *)
-  (*       simpl. splits*. *)
-  (*       * discriminate. *)
-  (*       * unfold pointer_of; simpl; trivial. *)
-  (*   - forwards (? & ?): IHys Hins. *)
-  (*     simpl. *)
-  (*     do 2 econstructor; eauto. *)
-  (*     + apply Clight.eval_Eaddrof. *)
-  (*       apply* Clight.eval_Evar_local. *)
-  (*     + apply sem_cast_same. *)
-  (*       splits*. *)
-  (*       * discriminate. *)
-  (*       * unfold pointer_of; simpl; trivial. *)
-  (* Qed. *)
-  
-  (* Theorem simu_bigbig: *)
-  (*   (forall p S1 s S2, *)
-  (*       stmt_eval p S1 s S2 -> *)
-  (*       sub_prog p prog -> *)
-  (*        forall c, *)
-  (*         In c prog -> *)
-  (*         forall e1 le1 m1 *)
-  (*           (WF: well_formed_stmt c S1 s)  *)
-  (*           (MS: match_states c S1 (e1, m1)), *)
-  (*         exists le2 m2 t, *)
-  (*           exec_stmt tge (Clight.function_entry1 tge) e1 le1 m1 *)
-  (*                     (translate_stmt c.(c_name) s) t le2 m2 ClightBigstep.Out_normal *)
-  (*           /\ match_states c S2 (e1, m2)) *)
-  (*   /\ (forall p me clsid vs me' rvs, *)
-  (*         stmt_step_eval p me clsid vs me' rvs -> *)
-  (*         sub_prog p prog -> *)
-  (*         forall c S o c' prog' m loc_f f loc_struct ofs e le outs, *)
-  (*           In c' prog -> *)
-  (*           well_formed_stmt c' (me, adds (Nelist.map_fst c'.(c_input)) vs v_empty) c'.(c_step) -> *)
-  (*           match_states c S (e, m) -> *)
-  (*           Globalenvs.Genv.find_symbol tge.(Clight.genv_genv) (step_id clsid) = Some loc_f -> *)
-  (*           Globalenvs.Genv.find_funct_ptr tge.(Clight.genv_genv) loc_f = Some (Ctypes.Internal f) -> *)
-  (*           find_inst S o me -> *)
-  (*           find_class clsid prog = Some (c', prog') -> *)
-  (*           List.length f.(Clight.fn_params) = 1 + Nelist.length vs + Nelist.length c'.(c_output) -> *)
-  (*           Clight.eval_expr tge e le m (ptr_obj (Some c.(c_name)) clsid o) (Values.Vptr loc_struct ofs) -> *)
-  (*           exists m' t, *)
-  (*             eval_funcall tge (Clight.function_entry1 tge) m (Ctypes.Internal f) *)
-  (*                          ((Values.Vptr loc_struct ofs) :: nelist2list vs ++ outs) t m' Values.Vundef *)
-  (*             /\ match_states c (update_inst S o me') (e, m') *)
-  (*       ). *)
-  (* Proof. *)
-  (*   clear TRANSL. *)
-  (*   apply stmt_eval_step_ind; *)
-  (*     [| |introv ? ? ? ? Hifte|introv ? HS1 ? HS2|introv ? Evs ? Hrec_eval| *)
-  (*      |(introv Hfind ? ? Hrec_exec; intros ** MS Hget_loc_f Hget_f ? Hfind' Hlengths ?)]; *)
-  (*     intros; *)
-  (*     try inverts WF as; [|introv Hin| | |introv Hlengths' Hins Hin Hfind Wfs ? Valids Types| |]; intros; *)
-  (*     inverts MS as Hvars Hself Hstep. *)
-
-  (*   (* Assign x e : "x = e" *) *)
-  (*   - app_exp_eval_det. *)
-  (*     edestruct Hvars; eauto. *)
-  (*     edestruct compat_assign_pres; iauto.   *)
-  (*     do 3 econstructor; split*. *)
-  (*     apply* ClightBigstep.exec_Sassign.  *)
-  (*     rewrite* type_pres. *)
-
-  (*   (* AssignSt x e : "self->x = e"*) *)
-  (*   - app_exp_eval_det. *)
-  (*     pose proof Hself as Hself'. *)
-  (*     destruct* Hself' as (? & ? & ? & ? & ? & ? & ? & Hmem & ?). *)
-  (*     specializes Hmem Hin; destruct_conjs.     *)
-  (*     edestruct compat_stassign_pres; iauto.       *)
-  (*     do 3 econstructor; split*. *)
-  (*     apply* ClightBigstep.exec_Sassign. *)
-  (*     + apply* evall_self_field.  *)
-  (*     + rewrite* type_pres. *)
-        
-  (*   (* Ifte e s1 s2 : "if e then s1 else s2" *) *)
-  (*   - edestruct Hifte with (le1:=le1); destruct_conjs; eauto; [destruct* b|].  *)
-  (*     do 3 econstructor; split*. *)
-  (*     apply* exec_Sifthenelse.  *)
-  (*     + erewrite type_pres, bool_val_ptr; eauto. *)
-  (*     + destruct* b.  *)
-      
-  (*   (* Comp s1 s2 : "s1; s2" *) *)
-  (*   - app_stmt_eval_det'. *)
-  (*     edestruct HS1; destruct_conjs; eauto. *)
-  (*     edestruct HS2; destruct_conjs; eauto. *)
-  (*     do 3 econstructor; split*. *)
-  (*     apply* exec_Sseq_1. *)
-
-  (*   (* Step_ap y ty clsid o [e1; ... ;en] : "y = clsid_step(&(self->o), e1, ..., en)" *) *)
-  (*   - app_exps_eval_det. *)
-  (*     app_find_inst_det. *)
-  (*     app_stmt_step_eval_det'. *)
-      
-  (*     (* get the Clight corresponding function *) *)
-  (*     forwards* Hin': find_class_In Hfind. *)
-  (*     pose proof Hstep as Hstep'. *)
-  (*     edestruct Hstep' as (loc_f & f & ? & ? & ? & Htype_fun & ? & ? & Hlengths & ?); eauto. *)
-  (*     rewrite <-type_pres' with (c:=c) (es:=es) (ys:=ys) in Htype_fun; auto. *)
-  (*     forwards Eq: find_class_name Hfind. *)
-  (*     rewrite Eq in *; clear Eq. *)
-      
-  (*     (* get the Clight corresponding field *) *)
-  (*     pose proof Hself as Hself'. *)
-  (*     destruct* Hself' as (? & ? & ? & ? & ? & ? & ? & ? & Hobj). *)
-  (*     specializes Hobj Hin; destruct Hobj.  *)
-
-  (*     (* get outs values *) *)
-  (*     edestruct exprlist_make_out_arg with (le:=le1) (c:=c) as (outs); eauto. *)
-      
-  (*     (* recursive funcall evaluation *) *)
-  (*     edestruct Hrec_eval with (c:=c) (e:=e1) (m:=m1) (le:=le1) (outs:=outs); destruct_conjs; eauto. *)
-  (*     + rewrite <-ne_Forall2_lengths with (1:=Evs). *)
-  (*       rewrite Hlengths; simpl; f_equal. *)
-  (*       rewrite app_length; do 2 rewrite <-nelist2list_length. *)
-  (*       f_equal; symmetry; apply* ne_Forall2_lengths.         *)
-  (*     + apply Clight.eval_Eaddrof; apply* evall_self_field. *)
-  (*     + do 3 econstructor; split*. *)
-  (*       *{ apply* exec_Scall. *)
-  (*          - simpl; eauto. *)
-  (*          - eapply Clight.eval_Elvalue. *)
-  (*            + apply* Clight.eval_Evar_global. *)
-  (*            + apply* Clight.deref_loc_reference. *)
-  (*          - econstructor. *)
-  (*            + eapply Clight.eval_Eaddrof. *)
-  (*              apply* evall_self_field. *)
-  (*            + eapply sem_cast_same. *)
-  (*              unfold valid_val; splits*. *)
-  (*              * discriminate. *)
-  (*              * simpl; trivial. *)
-  (*            + apply* eval_exprlist_app. *)
-  (*              apply* exprs_eval_simu. *)
-  (*          - eauto. *)
-  (*        } *)
-  (*       * admit.  *)
-
-  (*   (* Skip : "skip" *) *)
-  (*   - do 3 econstructor; split*. *)
-  (*     eapply exec_Sskip. *)
-
-  (*   (* funcall *) *)
-  (*   - forwards* Hfind'': find_class_sub_same Hfind UNIQUE. *)
-  (*     rewrite Hfind' in Hfind''; inverts Hfind''. *)
-  (*     destruct Hstep with (c:=cls) *)
-  (*       as (loc_f' & f' & Hget_loc_f' & Hget_f' & Htype_fun & Hvars_nil & ? & ? & Htr & ?); *)
-  (*       destruct_conjs; eauto. *)
-  (*     forwards Eq: find_class_name Hfind. *)
-  (*     rewrite Eq in Hget_loc_f'; clear Eq. *)
-  (*     rewrite Hget_loc_f' in Hget_loc_f; inverts Hget_loc_f. *)
-  (*     rewrite Hget_f' in Hget_f; inverts Hget_f. *)
-
-  (*     assert (length f.(Clight.fn_params) = length ((Values.Vptr loc_struct ofs) :: nelist2list vs)) *)
-  (*       by (rewrite Hlengths; simpl; f_equal; rewrite Nelist.nelist2list_length; auto). *)
-
-  (*     forwards* (le_fun & ? & ?): (compat_funcall_pres cls m). *)
-  (*     forwards* Hsub: find_class_sub. *)
-  (*     subst env. *)
-  (*     edestruct Hrec_exec with (le1:=le_fun) as (? & ? & ? & ? & MS); eauto. *)
-  (*     destruct_conjs. *)
-        
-  (*     do 2 econstructor; split. *)
-  (*     apply* eval_funcall_internal. *)
-  (*     + constructor*; rewrite Hvars_nil; simpl; constructor. *)
-  (*     + rewrite* Htr. *)
-  (*       apply* exec_Sseq_1. *)
-  (*       apply* exec_Sreturn_some. *)
-  (*       apply* Clight.eval_Etempvar. *)
-  (*       inverts MS as Hvars'. *)
-  (*       apply* Hvars'; rewrite <-surjective_pairing; eapply in_eq. *)
-  (*     + simpl; split*. *)
-  (*       inverts Htype_fun. *)
-  (*       apply* sem_cast_same. *)
-  (*     + simpl; eauto.        *)
-  (*     + constructor*. *)
-  (*       unfold compat_self. *)
-  (*       intro Hin. *)
-  (*       pose proof Hself as Hself'. *)
-  (*       destruct* Hself' as (? & loc_struct' & ofs' & Hget_self' & Hget_co' & Hmem & Hobj). *)
-  (*       do 3 econstructor; splits*. *)
-  (*       intros x' t' Hin'.  *)
-  (*       specializes Hmem Hin'; destruct Hmem. *)
-  (*       econstructor; splits*. *)
-  (*       * admit. *)
-  (*       * admit. *)
-  (* Qed. *)
