Simu/Sem.v
@@ -285,300 +285,62 @@ Ltac app_stmt_eval_det :=
     assert (S2 = S1) as H by (eapply stmt_eval_det; eauto); inverts H; clear H2
   end.
 
-(* Inductive sub_prog: program -> program -> Prop := *)
-(*   sub_prog_intro: forall p p', *)
-(*     sub_prog p (p' ++ p). *)
-
-(* Lemma find_class_sub: *)
-(*   forall prog clsid cls prog', *)
-(*     find_class clsid prog = Some (cls, prog') -> *)
-(*     sub_prog prog' prog. *)
-(* Proof. *)
-(*   introv Find. *)
-(*   forwards* (prog2' & ? & ?): find_class_app Find. *)
-(*   substs. *)
-(*   rewrite List_shift_first. *)
-(*   constructor. *)
-(* Qed. *)
-
-(* Hint Constructors sub_prog. *)
-
-(* Definition unique_classes (prog: program): Prop := *)
-(*   forall c1 c2, *)
-(*     List.In c1 prog -> *)
-(*     List.In c2 prog -> *)
-(*     c1.(c_name) <> c2.(c_name). *)
-
-(* Remark unique_nil : *)
-(*   unique_classes nil. *)
-(* Proof. *)
-(*   unfold unique_classes; intros; contradiction. *)
-(* Qed. *)
-
-(* Remark unique_cons: *)
-(*   forall cls c, *)
-(*     unique_classes (c :: cls) -> unique_classes cls. *)
-(* Proof. *)
-(*   destruct cls. *)
-(*   - intros; apply unique_nil. *)
-(*   - intros c' H. *)
-(*     unfold unique_classes. *)
-(*     introv Hin1 Hin2. *)
-(*     unfold unique_classes in H. *)
-(*     apply List.in_cons with (a:=c') in Hin1. *)
-(*     apply List.in_cons with (a:=c') in Hin2. *)
-(*     specializes H Hin1 Hin2. *)
-(* Qed. *)
-
-(* Remark unique_app: *)
-(*   forall cls cls', *)
-(*     unique_classes (cls ++ cls') -> unique_classes cls /\ unique_classes cls'. *)
-(* Proof. *)
-(*   induction cls. *)
-(*   - simpl; split; auto. apply unique_nil. *)
-(*   - intros cls' Unique. *)
-(*     split. *)
-(*     + unfold unique_classes. *)
-(*       introv Hin1 Hin2. *)
-(*       unfold unique_classes in Unique. *)
-(*       apply Unique; apply List.in_or_app; left; auto. *)
-(*     + rewrite <-List.app_comm_cons in Unique.   *)
-(*       apply unique_cons in Unique. *)
-(*       apply IHcls; auto. *)
-(* Qed. *)
-
-(* Remark find_class_sub_same: *)
-(*   forall prog1 prog2 clsid cls prog', *)
-(*     find_class clsid prog2 = Some (cls, prog') -> *)
-(*     unique_classes prog1 -> *)
-(*     sub_prog prog2 prog1 -> *)
-(*     find_class clsid prog1 = Some (cls, prog'). *)
-(* Proof. *)
-(*   introv Hfind Unique Sub. *)
-(*   inverts Sub. *)
-(*   forwards* (prog2' & Hprog2 & Hnone): find_class_app Hfind. *)
-(*   induction p'; simpl; auto. *)
-(*   rewrite <-List.app_comm_cons in Unique. *)
-(*   assert (List.In a (a :: p' ++ prog2)) as Hin_a by apply List.in_eq. *)
-(*   assert (List.In cls (a :: p' ++ prog2)) as Hin_cls. *)
-(*   - forwards* Hin: find_class_In Hfind. *)
-(*     rewrite List.app_comm_cons.    *)
-(*     apply List.in_or_app; right; auto.  *)
-(*   - forwards Neq: Unique Hin_a Hin_cls. *)
-(*     apply ident_eqb_neq in Neq. *)
-(*     forwards* Eq: find_class_name Hfind. *)
-(*     rewrite Eq in Neq; rewrite Neq. *)
-(*     apply IHp'. eapply unique_cons; eauto. *)
-(* Qed. *)
-
-(* Remark find_class_unique: *)
-(*   forall prog clsid cls prog', *)
-(*     unique_classes prog -> *)
-(*     find_class clsid prog = Some (cls, prog') -> *)
-(*     unique_classes prog'. *)
-(* Proof. *)
-(*   introv Unique Find. *)
-(*   forwards* (prog2' & Hprog2 & Hnone): find_class_app Find. *)
-(*   substs. *)
-(*   forwards (? & H): unique_app Unique. *)
-(*   eapply unique_cons; eauto. *)
-(* Qed. *)
-
-(* Lemma stmt_step_eval_det': *)
-(*   forall prog1 prog2 me clsid vs me1 rvs1 me2 rvs2, *)
-(*     unique_classes prog1 -> *)
-(*     stmt_step_eval prog1 me clsid vs me1 rvs1 -> *)
-(*     stmt_step_eval prog2 me clsid vs me2 rvs2 -> *)
-(*     sub_prog prog2 prog1 -> *)
-(*     me1 = me2 /\ rvs1 = rvs2. *)
-(* Proof. *)
-(*   introv Unique Hstp1; revert me2 rvs2 prog2. *)
-(*   induction Hstp1 using stmt_step_eval_ind_2 with *)
-(*   (P := fun p S s S' => unique_classes p -> forall S'', stmt_eval p S s S' -> stmt_eval p S s S'' -> S' = S''); *)
-(*     [| | | | | |introv Hstp2 Hsub]; try (introv Hev1 Hev2; inverts Hev2); try app_exp_eval_det; auto.  *)
-(*   - app_bool_val; auto. *)
-(*   - apply* IHHstp0. *)
-(*     asserts_rewrite* (S2 = S4). *)
-(*   - assert (omenv = omenv0) by apply* find_inst_det; subst omenv0. *)
-(*     assert (vs = vs0) by (eapply Forall2_det; eauto; eapply exp_eval_det); subst vs0. *)
-(*     repeat fequals; apply* IHHstp1; *)
-(*     rewrite* <-List.app_nil_l; simpl. *)
-(*   - inverts Hstp2. *)
-(*     substs. *)
-(*     forwards* H': find_class_sub_same. *)
-(*     rewrite H' in H; inverts H. *)
-(*     forwards Unique': find_class_unique Unique H'. *)
-(*     assert (S' = S'0); auto. subst S'0. *)
-(*     split*. *)
-(*     apply* find_vars_det. *)
-(* Qed. *)
-
-(* Ltac app_stmt_step_eval_det' := *)
-(*   match goal with *)
-(*   | H1: stmt_step_eval ?prog1 ?me ?clsid ?vs ?me1 ?rvs1, *)
-(*         H2: stmt_step_eval ?prog2 ?me ?clsid ?vs ?me2 ?rvs2,  *)
-(*             H3: sub_prog ?prog2 ?prog1, *)
-(*                 H4: unique_classes ?prog1 |- _ => *)
-(*     let H := fresh in *)
-(*     assert (me1 = me2 /\ rvs1 = rvs2) as H by (applys stmt_step_eval_det' H4 H1 H2 H3; eauto); inverts H; clear H2 *)
-(*   end. *)
-
-(* Theorem stmt_eval_det': *)
-(*   forall prog1 prog2 S s S1 S2, *)
-(*     unique_classes prog1 -> *)
-(*     stmt_eval prog1 S s S1 -> *)
-(*     stmt_eval prog2 S s S2 -> *)
-(*     sub_prog prog2 prog1 -> *)
-(*     S1 = S2. *)
-(* Proof. *)
-(*   intros until S2; intros Unique Hev1; revert S2; *)
-(*   induction Hev1; intros S2' Hev2 Hsub; inv Hev2; inv Hsub; *)
-(*   try app_exp_eval_det; auto. *)
-(*   - apply* IHHev1. *)
-(*     app_bool_val; eauto.     *)
-(*   - apply* IHHev1_2. *)
-(*     asserts_rewrite* (S2 = S4). *)
-(*   - assert (omenv = omenv0) by apply* find_inst_det; subst omenv0. *)
-(*     assert (vs = vs0) by (eapply Forall2_det; eauto; eapply exp_eval_det); subst vs0. *)
-(*     repeat fequals; apply* stmt_step_eval_det'. *)
-(* Qed. *)
-
-(* Ltac app_stmt_eval_det' := *)
-(*   match goal with *)
-(*   | H1: stmt_eval ?prog1 ?S ?s ?S1, *)
-(*         H2: stmt_eval ?prog2 ?S ?s ?S2, *)
-(*             H3: sub_prog ?prog2 ?prog1, *)
-(*                 H4: unique_classes ?prog1 |- _ => *)
-(*     let H := fresh in *)
-(*     assert (S1 = S2) as H by (applys stmt_eval_det' H4 H1 H2 H3; eauto); inverts H; clear H2 *)
-(*   end. *)
-
-(* Inductive cont := *)
-(* | Kstop: cont *)
-(* | Kseq: stmt -> cont -> cont. *)
-
-(* (* =stmt_eval= *) *)
-(* Inductive stmt_eval_cont: state * stmt * cont -> state * stmt * cont -> Prop := *)
-(* | Iassign_cont: forall me ve x e v ve' k, *)
-(*     exp_eval me ve e v -> *)
-(*     PM.add x v ve = ve' -> *)
-(*     stmt_eval_cont ((me, ve), Assign x e, k) ((me, ve'), Skip, k) *)
-(* | Iassignst_cont: forall me ve x e v me' k, *)
-(*     exp_eval me ve e v -> *)
-(*     madd_mem x v me = me' -> *)
-(*     stmt_eval_cont ((me, ve), AssignSt x e, k) ((me', ve), Skip, k) *)
-(* | Iifte_cont: forall me ve m e v b s1 s2 k, *)
-(*     exp_eval me ve e v -> *)
-(*     (forall ty attr, Ctypes.typeconv (typeof e) <> Ctypes.Tpointer ty attr) -> *)
-(*     Cop.bool_val v (typeof e) m = Some b -> *)
-(*     stmt_eval_cont ((me, ve), Ifte e s1 s2, k) ((me, ve), if b then s1 else s2, k)     *)
-(* | Icomp_cont: forall st s1 s2 k, *)
-(*     stmt_eval_cont (st, Comp s1 s2, k) (st, s1, Kseq s2 k) *)
-(* | Iskip_comp_cont: forall st s k, *)
-(*     stmt_eval_cont (st, Skip, Kseq s k) (st, s, k). *)
-
-(* Section SEQUENCES. *)
-(*   Set Implicit Arguments. *)
-
-(*   Variable A: Type.  *)
-(*   Variable R: A -> A -> Prop.  *)
-
-(*   Inductive star: A -> A -> Prop := *)
-(*   | star_refl: forall a, *)
-(*       star a a *)
-(*   | star_step: forall a b c, *)
-(*       R a b -> star b c -> star a c. *)
-
-(*   Hint Constructors star. *)
-
-(*   Lemma star_one: *)
-(*     forall (a b: A), R a b -> star a b. *)
-(*   Proof. *)
-(*     intros. econstructor; eauto.  *)
-(*   Qed. *)
-
-(*   Lemma star_trans: *)
-(*     forall (a b: A), star a b -> forall c, star b c -> star a c. *)
-(*   Proof. *)
-(*     induction 1; intros. auto. econstructor; eauto. *)
-(*   Qed. *)
-
-(*   Lemma one_star_trans: *)
-(*     forall (a b: A), R a b -> forall c, star b c -> star a c. *)
-(*   Proof. *)
-(*     intros. econstructor; eauto. *)
-(*   Qed. *)
-
-(* End SEQUENCES. *)
-
-(* Definition terminates (S: state) (s: stmt) (S': state) : Prop := *)
-(*   star stmt_eval_cont (S, s, Kstop) (S', Skip, Kstop). *)
-
-(* Hint Resolve star_one star_trans one_star_trans.  *)
-(* Hint Constructors star stmt_eval_cont. *)
-
-(* Theorem to_cont: *)
-(*   forall S s S', *)
-(*     stmt_eval S s S' -> *)
-(*     forall k, star stmt_eval_cont (S, s, k) (S', Skip, k). *)
-(* Proof. *)
-(*   induction 1; eauto. *)
-(* Qed. *)
-
-
-(* Inductive keval: cont -> state -> state -> Prop := *)
-(* | KE_stop: forall S, *)
-(*     keval Kstop S S *)
-(* | KE_seq: forall s k S S' S'', *)
-(*     stmt_eval S s S' -> *)
-(*     keval k S' S'' -> *)
-(*     keval (Kseq s k) S S''. *)
-
-(* Inductive skeval: state * stmt * cont -> state -> Prop := *)
-(*   ske_intro: forall s k S S' S'', *)
-(*       stmt_eval S s S' -> *)
-(*       keval k S' S'' -> *)
-(*       skeval (S, s, k) S''. *)
-
-(* Require Import Coq.Program.Equality. *)
-
-(* Hint Constructors stmt_eval. *)
-
-(* Lemma stmt_eval_cont_skeval: *)
-(*   forall S s k S' s' k', *)
-(*     stmt_eval_cont (S, s, k) (S', s', k') -> *)
-(*     forall S'', *)
-(*       skeval (S', s', k') S'' -> *)
-(*       skeval (S, s, k) S''. *)
-(* Proof. *)
-(*   intros until k'. intro STEP. dependent induction STEP; intros. *)
-(*   - inv H0. inv H5. econstructor; eauto; auto. *)
-(*   - inv H0. inv H5. econstructor; eauto; auto. *)
-(*   - inv H2. destruct S'. econstructor. econstructor; eauto. auto. *)
-(*   - inv H. inv H5. econstructor; eauto. destruct S', S'1, S'0. econstructor; eauto. *)
-(*   - inv H. econstructor; eauto. econstructor; eauto. *)
-(* Qed. *)
-
-(* Lemma stmt_eval_cont_skeval': *)
-(*   forall S s k S' s' k' S'', *)
-(*     star stmt_eval_cont (S, s, k) (S', s', k') -> *)
-(*     skeval (S', s', k') S'' -> *)
-(*     skeval (S, s, k) S''. *)
-(* Proof. *)
-(*   intros; dependent induction H; auto. *)
-(*   destruct b as [[S1 s1] k1]. *)
-(*   eapply stmt_eval_cont_skeval; eauto. *)
-(* Qed. *)
-
-(* Hint Constructors keval. *)
-
-(* Theorem from_cont: *)
-(*   forall S s S', *)
-(*   terminates S s S' -> stmt_eval S s S'. *)
-(* Proof. *)
-(*   unfold terminates; intros. *)
-(*   assert (SKEV: skeval (S, s, Kstop) S'). *)
-(*   - eapply stmt_eval_cont_skeval'; eauto. *)
-(*     econstructor; eauto.  *)
-(*   - inv SKEV. inv H5; auto. *)
-(* Qed. *)
+Lemma stmt_step_eval_det': 
+  forall prog1 prog2 me clsid f vs me1 rvs1 me2 rvs2, 
+    WelldefClasses prog1 -> 
+    stmt_call_eval prog1 me clsid f vs me1 rvs1 -> 
+    stmt_call_eval prog2 me clsid f vs me2 rvs2 -> 
+    sub_prog prog2 prog1 -> 
+    me1 = me2 /\ rvs1 = rvs2. 
+Proof. 
+  introv WD Hstp1; revert me2 rvs2 prog2. 
+  induction Hstp1 using stmt_call_eval_ind_2 with 
+  (P := fun p S s S' => WelldefClasses p -> forall S'', stmt_eval p S s S' -> stmt_eval p S s S'' -> S' = S''); 
+    [| | | | | |introv Hstp2 Hsub]; try (introv Hev1 Hev2; inverts Hev2); try app_exp_eval_det; auto.  
+  - app_bool_val; auto. 
+  - apply* IHHstp0. 
+    asserts_rewrite* (S2 = S4). 
+  - assert (omenv = omenv0) by apply* find_inst_det; subst omenv0. 
+    assert (vs = vs0) by (eapply Forall2_det; eauto; eapply exp_eval_det); subst vs0. 
+    repeat fequals; apply* IHHstp1; 
+    rewrite* <-List.app_nil_l; simpl. 
+  - inverts Hstp2. 
+    forwards* H': find_class_sub_same. 
+    rewrite H' in H; inverts H. 
+    rewrite H0 in H4; inverts H4.
+    forwards WD': find_class_welldef WD H'. 
+    assert (S' = S'0); auto.
+    subst S'0. 
+    split*. 
+    apply* find_vars_det. 
+Qed. 
+ 
+Theorem stmt_eval_det': 
+  forall prog1 prog2 S s S1 S2, 
+    WelldefClasses prog1 -> 
+    stmt_eval prog1 S s S1 -> 
+    stmt_eval prog2 S s S2 -> 
+    sub_prog prog2 prog1 -> 
+    S1 = S2. 
+Proof. 
+  intros until S2; intros WD Hev1; revert S2; 
+  induction Hev1; intros S2' Hev2 Hsub; inverts Hev2; inverts Hsub; 
+  try app_exp_eval_det; auto. 
+  - apply* IHHev1. 
+    app_bool_val; eauto.     
+  - apply* IHHev1_2. 
+    asserts_rewrite* (S2 = S4). 
+  - assert (omenv = omenv0) by apply* find_inst_det; subst omenv0. 
+    assert (vs = vs0) by (eapply Forall2_det; eauto; eapply exp_eval_det); subst vs0. 
+    repeat fequals; apply* stmt_step_eval_det'. 
+Qed. 
+ 
+Ltac app_stmt_eval_det' := 
+  match goal with 
+  | H1: stmt_eval ?prog1 ?S ?s ?S1, 
+        H2: stmt_eval ?prog2 ?S ?s ?S2, 
+            H3: sub_prog ?prog2 ?prog1, 
+                H4: WelldefClasses ?prog1 |- _ => 
+    let H := fresh in 
+    assert (S1 = S2) as H by (applys stmt_eval_det' H4 H1 H2 H3; eauto); inverts H; clear H2 
+  end.
